# 5.4.2 来自常规语法的正则表达式

Occasionally, for example in Section 9.12, it is useful to condense a regular grammar into a regular expression. The transformation can be performed by alternatingly sub- stituting a rule and applying the transformation patterns from Figure 5.19. The first pattern combines all rules for the same non-terminal. The second pattern combines all regular expressions that precede the same non-terminal in a right-hand side; α is a list of alternatives that do not end in Q (but see next paragraph). The third pat- tern removes right recursion: if the repetitive part is (R), it prepends (R)∗ to all non- recursive alternatives; here β consists of all the alternatives in α, with (R)∗ prepended to each of them. Q1, Q2, ··· should not be equal to P (but see next paragraph). When α is ε it can be left out when it is concatenated with a non-empty regular expression.

![图1](../../img/5.4.2_1-Fig.5.19.png)

The substitutions and transformations may be applied in any order and will al- ways lead to a correct regular expression, but the result depends heavily on the appli- cation order; to obtain a “nice” regular expression, human guidance is needed. Also, the two conditions in the previous paragraph may be violated without endangering the correctness, but the result will be a more “ugly” regular expression.

We will now apply the transformation to the regular grammar of Figure 5.18, and will not hesitate to supply the human guidance. We first combine the rules by their left-hand sides (transformation 1):

**<center>S -> A<center>**
**<center>A -> aB|pC|qC<center>**
**<center>B -> b A<center>**
**<center>C -> pC|qC| ε<center>**

Next we substitute B:

**<center>A -> abA|pC|qC<center>**
**<center>C -> pC|qC| ε<center>**

followed by scooping up prefixes (transformation 2):

**<center>A -> (ab) A | (p|q) C<center>**
**<center>C -> (p|q)C| ε<center>**

Note that we have also packed the ab that prefixes A, to prepare it for the next transformation, which involves turning recursion into repetition:

**<center>S -> A<center>**
**<center>A -> (ab)<sub>*</sub> (p|q) C<center>**
**<center>C -> (p|q)<sub>*</sub><center>**

Now C can be substituted in A and A in S, resulting in

**<center>S -> (ab)<sub>*</sub> (p|q) (p|q)<sub> *</sub><center>**

This is equivalent but not identical to the (ab)*(p|q)+ we started with.